---
title: "Prove H and I-H are Idempotent"
date: "2021-11-29"
categories: [Proof, Statistics, Linear Regression]
toc: true
---

Define the hat matrix $H=X(X^TX)^{-1}X^T$. Prove H and I-H are Idempotent

![](idempotent.png)

# `Proof`

For H to be Idempotent then $HH=H$

\begin{equation}\label{HH=H}
\begin{split}
HH & =[X(X^TX)^{-1}X^T][X(X^TX)^{-1}X^T]\\
& = X(X^TX)^{-1}X^TX(X^TX)^{-1}X^T\quad\quad(X^TX)^{-1}X^TX=1\\
& = X(X^TX)^{-1}X^T\\
& = H
\end{split}
\end{equation}

Therefore by the series of equalities H is idempotent. 

For I-H to be idempotent then $(I-H)(I-H)=I-H$

\begin{equation}\label{I-H}
\begin{split}
(I-H)(I-H) & =II-HI-IH+HH\quad\quad II=I, HI=IH=H, HH=H\\
& = I-H-H+H\\
& = I-H
\end{split}
\end{equation}

Therefor by the series of equalities I-H is idempotent. 

QED. 
